\documentclass[a4paper,12pt]{article}
\usepackage[T1]{fontenc}
\usepackage[utf8]{inputenc}
\usepackage{amssymb}
\usepackage[polish]{babel}
\usepackage{amsmath}
\usepackage{times}
\usepackage{anysize}
\usepackage{array}

\marginsize{1.5cm}{1.5cm}{1.5cm}{1.5cm}
\sloppy 


\begin{document}

$$\int\limits_{-1}^2 (x^2 - 2x) dx =\left|
	\begin{array}{c}
	f(x) = x^2 - 2x \\
	\int f(x)dx = \cfrac{x^3}{3} - x^2 + C \\
	F(x) = \cfrac{x^3}{3} - x^2
	\end{array}
	\right|
= \left[
	\begin{array}{c}
	\cfrac{x^3}{3} - x^2
	\end{array}
	\right]_{-1}^2
$$

$$ = \left(
	\begin{array}{c}
{\cfrac{2^3}{3} - 2^2}
	\end{array}
	\right)
 - \left(
	\begin{array}{c}
	\cfrac{(-1)^3}{3} - (-1)^2
	\end{array}
	\right) 
= \left(
	\begin{array}{c}
\cfrac{8}{3} - 4
	\end{array}
	\right)
 - \left(
	\begin{array}{c}
	-\cfrac{1}{3} - 1
	\end{array}
	\right)
 = -\frac{4}{3} + \frac{4}{3} = 0 $$

\end{document}
